progerss assert proof generation metatheory, allow steps in Boogie program at beginning of method call rule

ViperBoogieRelUtil.thy
@@ -1147,9 +1147,9 @@ definition pred_eq_heap
                                     total_heap_well_typed Pr (domain_type TyRep) (get_hh_total_full \<omega>)"
 
 definition aux_pred_capture_state
-  where "aux_pred_capture_state Pr TyRep Tr AuxPred ctxt m h \<omega> \<equiv>
-           AuxPred(m \<mapsto> pred_eq_mask Pr TyRep (field_translation Tr) ctxt m \<omega>)
-                  (h \<mapsto> pred_eq_heap Pr TyRep (field_translation Tr) ctxt h \<omega>)"
+  where "aux_pred_capture_state Pr TyRep FieldTr AuxPred ctxt m h \<omega> \<equiv>
+           AuxPred(m \<mapsto> pred_eq_mask Pr TyRep FieldTr ctxt m \<omega>)
+                  (h \<mapsto> pred_eq_heap Pr TyRep FieldTr ctxt h \<omega>)"
 
 lemma aux_pred_capture_state_dom: 
   "dom (aux_pred_capture_state Pr TyRep Tr AuxPred ctxt m h \<omega>) = dom AuxPred \<union> {m,h}"
@@ -1163,18 +1163,19 @@ abbreviation state_rel_capture_total_state :: \<comment>\<open>make type explici
      \<Rightarrow> ('a full_total_state \<Rightarrow> bool)
         \<Rightarrow> 'a ty_repr_bpl
            \<Rightarrow> tr_vpr_bpl
+             \<Rightarrow> (field_ident \<rightharpoonup> Lang.vname)
               \<Rightarrow> (nat \<Rightarrow> ('a vbpl_absval Semantics.val \<Rightarrow> bool) option)
                  \<Rightarrow> ('a vbpl_absval, 'b) econtext_bpl_general_scheme \<Rightarrow> nat \<Rightarrow> nat \<Rightarrow> 'a full_total_state \<Rightarrow> 'a full_total_state \<Rightarrow> 'a full_total_state \<Rightarrow> 'a vbpl_absval nstate \<Rightarrow> bool"
-  where "state_rel_capture_total_state Pr StateCons TyRep Tr AuxPred ctxt m h \<omega> \<equiv> 
+  where "state_rel_capture_total_state Pr StateCons TyRep Tr FieldTr0 AuxPred ctxt m h \<omega> \<equiv> 
           state_rel Pr StateCons TyRep Tr 
-                         (aux_pred_capture_state Pr TyRep Tr AuxPred ctxt m h \<omega>)
+                         (aux_pred_capture_state Pr TyRep FieldTr0 AuxPred ctxt m h \<omega>)
                          ctxt"
 
 lemma state_rel_capture_total_stateI:
   assumes "state_rel Pr StateCons TyRep Tr AuxPred' ctxt \<omega>def \<omega> ns"
-      and "AuxPred' = (AuxPred(m \<mapsto> pred_eq_mask Pr TyRep (field_translation Tr) ctxt m \<omega>0)
-                              (h \<mapsto> pred_eq_heap Pr TyRep (field_translation Tr) ctxt h \<omega>0))"
-    shows "state_rel_capture_total_state Pr StateCons TyRep Tr AuxPred ctxt m h \<omega>0 \<omega>def \<omega> ns"
+      and "AuxPred' = (AuxPred(m \<mapsto> pred_eq_mask Pr TyRep FieldTr0 ctxt m \<omega>0)
+                              (h \<mapsto> pred_eq_heap Pr TyRep FieldTr0 ctxt h \<omega>0))"
+    shows "state_rel_capture_total_state Pr StateCons TyRep Tr FieldTr0 AuxPred  ctxt m h \<omega>0 \<omega>def \<omega> ns"
   using assms
   unfolding aux_pred_capture_state_def
   by simp
@@ -1456,8 +1457,9 @@ proof -
 qed
 
 lemma state_rel_capture_total_state_change_eval_state:
-  assumes StateRel: "state_rel_capture_total_state Pr StateCons TyRep Tr' AuxPred ctxt m h \<omega>0 \<omega>def \<omega> ns"      
+  assumes StateRel: "state_rel_capture_total_state Pr StateCons TyRep Tr' FieldTr0 AuxPred ctxt m h \<omega>0 \<omega>def \<omega> ns"      
       and "m \<noteq> h"
+      and "field_translation Tr' = FieldTr0"
       and DisjAuxPred: "{m,h} \<inter> dom AuxPred = {}"
       and "\<omega>0 = \<omega>def"
       and "Tr = Tr'\<lparr>mask_var := m, heap_var := h, mask_var_def := m, heap_var_def := h\<rparr>"
