StmtRelML.thy
@@ -263,6 +263,7 @@ ML \<open>
     (Rmsg' "stmt rel assert propagate progress" (resolve_tac ctxt @{thms red_ast_bpl_rel_transitive} THEN' (progress_red_bpl_rel_tac ctxt)) ctxt) THEN'
 (*    (Rmsg' "stmt rel assert track well-def" (resolve_tac ctxt [@{thm red_ast_bpl_rel_weaken_input} OF @{thms state_rel_def_same_to_state_rel}] THEN' assm_full_simp_solved_tac ctxt) ctxt) THEN'*)
     (Rmsg' "stmt rel assert setup well-def state exhale" ((#setup_well_def_state_tac hint) (#basic_info info) ctxt) ctxt) THEN'
+    (K (print_tac ctxt "after setup well def assert")) THEN'
     (Rmsg' "stmt rel assert exhale rel post propagate" (resolve_tac ctxt @{thms exhale_rel_propagate_posts_same_exh}) ctxt) THEN'
      exhale_rel_aux_tac ctxt info (#exhale_rel_hint hint) THEN'
     (Rmsg' "stmt rel assert exhale rel revert well-def vars" (exhale_revert_state_relation ctxt (#basic_info info)) ctxt) THEN'
@@ -272,11 +273,14 @@ ML \<open>
     
     (Rmsg' "assert rel mask and heap var" (assm_full_simp_solved_with_thms_tac [#tr_def_thm basic_info] ctxt) ctxt) THEN'
     (Rmsg' "assert rel invariant" (assm_full_simp_solved_tac ctxt) ctxt) THEN'
-    (Rmsg' "assert rel setup assert propagate" (resolve_tac ctxt @{thms exhale_rel_propagate_pre_no_inv_same_exh}) ctxt) THEN'
+    (Rmsg' "assert rel setup assert propagate" (resolve_tac ctxt @{thms exhale_rel_propagate_pre_no_inv}) ctxt) THEN'
     (Rmsg' "assert rel setup assert state tac" 
-              (EVERY'_red_ast_bpl_rel_transitive_with_inv_fst_eq_snd ctxt (map (fn tac => tac basic_info) setup_assert_state_tacs)) ctxt) THEN'
+          ( EVERY'_red_ast_bpl_rel_transitive_custom ctxt 
+            @{thm red_ast_bpl_rel_transitive_with_inv_capture_state[where ?Q="\<lambda>\<omega>. fst \<omega> = snd \<omega>"]}
+           (map (fn tac => tac basic_info) setup_assert_state_tacs)) ctxt) THEN'
     (Rmsg' "assert rel show state rel capture init 1" (resolve_tac ctxt @{thms red_ast_bpl_rel_input_implies_output}) ctxt) THEN'
-    (Rmsg' "assert rel show state rel capture init 2" (state_rel_capture_state_intro ctxt) ctxt)      
+    (Rmsg' "assert rel show state rel capture init 2" (state_rel_capture_state_intro ctxt) ctxt) THEN'
+    (Rmsg' "assert rel exhale rel capture state abstract" (resolve_tac ctxt @{thms exhale_rel_capture_state_abstract}) ctxt)
                  
   fun atomic_rel_inst_tac ctxt (inhale_info: atomic_inhale_rel_hint inhale_rel_info) (exhale_info: atomic_exhale_rel_hint exhale_rel_info) (basic_info : basic_stmt_rel_info) (atomic_hint : atomic_rel_hint)  = 
     (case atomic_hint of 
@@ -294,12 +298,13 @@ ML \<open>
         (Rmsg' "AtomicExh3 Invariant" (assm_full_simp_solved_tac ctxt) ctxt) THEN'
         (exhale_rel_tac ctxt exhale_info exh_complete_hint)
      | AssertHint assert_complete_hint =>
+        (K (print_tac ctxt "before assert tac")) THEN'
         (Rmsg' "AtomicAssert Start" (resolve_tac ctxt [#assert_stmt_rel_thm assert_complete_hint]) ctxt) THEN'
-        (Rmsg' "AtomicAssert Init" ((#init_tac assert_complete_hint) basic_info ctxt) ctxt) THEN'         
+        (Rmsg' "AtomicAssert Init" ((#init_tac assert_complete_hint) basic_info ctxt) ctxt) THEN' 
         (assert_rel_tac ctxt exhale_info assert_complete_hint)
      | MethodCallHint (callee_name, rets_lookup_decl_thms, inhale_info_call, exhale_info_call, exh_pre_complete_hint, inh_post_complete_hint) => 
         let val callee_data = Symtab.lookup (#method_data_table basic_info) callee_name |> Option.valOf in
-        (Rmsg' "MethodCall Start" (resolve_tac ctxt [@{thm method_call_stmt_rel} OF [#consistency_wf_thm basic_info, #consistency_down_mono_thm basic_info]]) ctxt) THEN'
+        (Rmsg' "MethodCall Start" (resolve_tac ctxt [@{thm method_call_stmt_rel_inst} OF [#consistency_wf_thm basic_info, #consistency_down_mono_thm basic_info]]) ctxt) THEN'
         (Rmsg' "MethodCall Program Eq" (assm_full_simp_solved_tac ctxt) ctxt) THEN'
         (Rmsg' "MethodCall ConsistencyEnabled" (assm_full_simp_solved_with_thms_tac [#tr_def_thm basic_info, @{thm default_state_rel_options_def}] ctxt) ctxt) THEN'
         (Rmsg' "MethodCall MdeclSome" (assm_full_simp_solved_with_thms_tac [#method_lookup_thm callee_data] ctxt) ctxt) THEN'
